src/fstar/FStarC.OCaml.fsti
@@ -24,15 +24,23 @@ val shellescape (s:string) : string
 This is NOT escaped. *)
 val new_ocamlpath () : string
 
-(* Run a command with the new OCAMLPATH set. The cmd is usually args[0], in Unix convention.
-This calls execvp, so it will not return if successful. Raises a Failure if the execvp fails.
-It also tries to find the command in the PATH, absolute path is not needed. *)
+(* Run a command with the new OCAMLPATH set. This calls execvp, so it
+will not return if successful. Raises a Failure if the execvp fails. It
+also tries to find the command in the PATH, absolute path is not needed.
+*)
 val exec_in_ocamlenv (#a:Type) (cmd : string) (args : list string) : a
 
-(* Run ocamlc passing appropriate flags to generate an executable. Expects
-the source file and further options as arguments. *)
+(* Run ocamlc (i.e. bytecode compiler) passing appropriate flags to
+generate a bytecode executable. Expects the source file and further
+options as arguments. *)
 val exec_ocamlc #a (args : list string) : a
 
-(* Run ocamlc passing appropriate flags to generate an F* plugin, using
-fstar_plugin_lib. Expects the source file and further options as arguments. *)
-val exec_ocamlc_plugin #a (args : list string) : a
+(* Run ocamlopt (i.e. native compiler) passing appropriate flags to
+generate an executable. Expects the source file and further options as
+arguments. *)
+val exec_ocamlopt #a (args : list string) : a
+
+(* Run ocamlc passing appropriate flags to generate an F* plugin,
+using fstar_plugin_lib. Expects the source file and further options as
+arguments. *)
+val exec_ocamlopt_plugin #a (args : list string) : a
